@@ -1,0 +1,917 @@
+
+Require Import LibTactics.
+Require Import Arith.
+Require Import Lia.
+From Coq Require Import Strings.String.
+Require Import Coq.Lists.List.
+Require Import Coq.Classes.EquivDec.
+
+
+Inductive typ :=
+  | int : typ
+  | top : typ
+  | arr : typ -> typ -> typ
+  | and : typ -> typ -> typ
+  | rcd : string -> typ -> typ.
+
+Inductive op := app | box | mrg.
+
+Inductive exp :=
+  | ctx : exp
+  | lit : nat -> exp
+  | unit : exp
+  | binop : op -> exp -> exp -> exp 
+  | lam : typ -> exp -> exp
+  | proj: exp -> nat -> exp
+  | clos: exp -> typ -> exp -> exp
+  | rec : string -> exp -> exp
+  | rproj : exp -> string -> exp.
+
+Inductive lookup : typ -> nat -> typ -> Prop :=
+  | lzero : forall A B, 
+      lookup (and A B) 0 B
+  | lsucc : forall A B n C, 
+      lookup A n C -> 
+      lookup (and A B) (S n) C.
+
+Inductive value : exp -> Prop :=
+  | vint : forall n, value (lit n)
+  | vunit : value unit
+  | vclos : forall v A e, value v -> value (clos v A e)
+  | vrcd : forall l v, value v -> value (rec l v)
+  | vmrg : forall v1 v2, value v1 -> value v2 -> value (binop mrg v1 v2).
+
+Inductive lin: string -> typ -> Prop :=
+  | lin_rcd: forall A l, lin l (rcd l A)
+  | lin_andl: forall A B l,
+      lin l A ->
+      lin l (and A B)
+  | lin_andr: forall A B l,
+     lin l B ->
+     lin l (and A B).
+
+Inductive rlookup : typ -> string -> typ -> Prop :=
+  | rlzero : forall l B, 
+      rlookup (rcd l B) l B
+  | landl : forall A B C l, 
+      rlookup A l C ->
+      ~ lin l B ->
+      rlookup (and A B) l C
+  | landr : forall A B C l, 
+      rlookup B l C ->
+      ~ lin l A ->
+      rlookup (and A B) l C.
+
+Inductive has_type : typ -> exp -> typ -> Prop :=
+  | tctx: forall E, has_type E ctx E
+  | tint : forall E i, has_type E (lit i) int
+  | tunit : forall E, has_type E unit top
+  | tapp : forall E A B e1 e2,
+      has_type E e1 (arr A B) -> has_type E e2 A -> has_type E (binop app e1 e2) B
+  | tbox : forall E A E1 e1 e2,
+      has_type E e1 E1 -> has_type E1 e2 A -> has_type E (binop box e1 e2) A
+  | tmrg : forall E e1 e2 A B,
+      has_type E e1 A -> has_type (and E A) e2 B -> has_type E (binop mrg e1 e2) (and A B)
+  | tlam : forall E A e B,
+      has_type (and E A) e B -> has_type E (lam A e) (arr A B)
+  | tproj: forall E A e B n,
+      has_type E e A ->
+      lookup A n B ->
+      has_type E (proj e n) B
+  | tclos : forall E E1 A e ev B, 
+      value ev ->
+      has_type top ev E1 -> 
+      has_type (and E1 A) e B -> 
+      has_type E (clos ev A e) (arr A B)
+  | trcd : forall E e A l,
+      has_type E e A ->
+      has_type E (rec l e) (rcd l A)
+  | trproj : forall E e B l A,
+      has_type E e B ->
+      rlookup B l A ->
+      has_type E (rproj e l) A.
+  
+Inductive lookupv : exp -> nat -> exp -> Prop :=
+  | lvzero : forall v1 v2, 
+      lookupv (binop mrg v1 v2) 0 v2
+  | lvsucc : forall v1 v2 n v3, 
+      lookupv v1 n v3 -> 
+      lookupv (binop mrg v1 v2) (S n) v3.
+
+Inductive rlookupv : exp -> string -> exp -> Prop :=
+  | rvlzero : forall l e, 
+      rlookupv (rec l e) l e
+  | vlandl : forall e1 e2 e l, 
+      rlookupv e1 l e ->
+      rlookupv (binop mrg e1 e2) l e
+  | vlandr : forall e1 e2 e l, 
+      rlookupv e2 l e ->
+      rlookupv (binop mrg e1 e2) l e.
+
+Inductive step : exp -> exp -> exp -> Prop :=
+  | sctx: forall v,
+      value v ->
+      step v ctx v
+  | sbl : forall v e1 e2 e1' o,
+      value v -> 
+      step v e1 e1' -> 
+      step v (binop o e1 e2) (binop o e1' e2)
+  | sbapp : forall v v1 e2 e2', 
+      value v -> 
+      value v1 -> 
+      step v e2 e2' -> 
+      step v (binop app v1 e2) (binop app v1 e2')
+  | sbbox : forall v v1 e2 e2', 
+      value v -> 
+      value v1 -> 
+      step v1 e2 e2' -> 
+      step v (binop box v1 e2) (binop box v1 e2')
+  | sbmrg : forall v v1 e' e,
+      value v -> 
+      value v1 -> 
+      step (binop mrg v v1) e e' -> 
+      step v (binop mrg v1 e) (binop mrg v1 e')
+  | sclos : forall v A e, 
+      value v -> 
+      step v (lam A e) (clos v A e)
+  | sbeta : forall v v1 v2 A e, value v -> value v1 -> value v2 -> 
+      step v (binop app (clos v2 A e) v1) (binop box (binop mrg v2 v1) e)
+  | sboxv : forall v v1 v2,
+      value v -> 
+      value v1 -> 
+      value v2 -> 
+      step v (binop box v1 v2) v2
+  | sproj: forall v e1 e2 n,
+      value v ->
+      step v e1 e2 ->
+      step v (proj e1 n) (proj e2 n)
+  | sprojv : forall v n v1 v2, 
+      value v ->
+      value v1 ->
+      lookupv v1 n v2 ->
+      step v (proj v1 n) v2
+  | srec: forall v e1 e2 l,
+      value v ->
+      step v e1 e2 ->
+      step v (rec l e1) (rec l e2)
+  | srproj: forall v e1 e2 l,
+      value v ->
+      step v e1 e2 ->
+      step v (rproj e1 l) (rproj e2 l)
+  | srprojv : forall v l v1 v2, 
+      value v ->
+      value v1 ->
+      rlookupv v1 l v2 ->
+      step v (rproj v1 l) v2.
+
+#[export]
+Hint Constructors typ op exp lookup lookupv lin rlookup has_type value rlookupv step : core.
+
+
+Require Import Program.Equality.
+
+
+(* ---------------------------------------------------- *)
+(* Type soundness *)
+Lemma value_weaken : forall E v A, 
+  has_type E v A -> forall E', 
+  value v -> 
+  has_type E' v A.
+Proof.
+  introv Ht. inductions Ht; introv Hv;
+  try solve [eauto];
+  try solve [inverts* Hv].
+Qed.
+
+Lemma lookupv_value: forall v n v', 
+  lookupv v n v' -> 
+  value v -> 
+  value v'.
+Proof.
+  introv Hl. inductions Hl; introv Hv; inverts* Hv.
+Qed.
+
+Lemma lookup_pres_ctx: forall E n A,
+  lookup E n A -> forall v v',
+  lookupv v n v' -> 
+  value v ->
+  has_type top v E ->
+  has_type E v' A.
+Proof.
+  introv Hl. inductions Hl; introv Hlv Hv Ht.
+  - inverts* Hlv. inverts* Ht. inverts Hv.
+    eapply value_weaken; eauto.
+  - inverts* Hlv. inverts* Ht. inverts Hv.
+    forwards~: IHHl H1 H2.
+    eapply value_weaken; eauto.
+    eapply lookupv_value; eauto.
+Qed.
+
+Lemma lookup_pres: forall E n A,
+  lookup E n A -> forall v v',
+  lookupv v n v' -> 
+  value v ->
+  has_type top v E ->
+  has_type top v' A.
+Proof.
+  introv Hl Hlv Hv Ht.
+  forwards~: lookup_pres_ctx Hl Hlv Hv Ht.
+  eapply value_weaken; eauto.
+  eapply lookupv_value; eauto. 
+Qed.
+
+
+Lemma rlookupv_value: forall v l v', 
+  rlookupv v l v' -> 
+  value v -> 
+  value v'.
+Proof.
+  introv Hl. inductions Hl; introv Hv; inverts* Hv.
+Qed.
+
+
+Lemma rcd_shape: forall E v l B, 
+  has_type E v (rcd l B) -> 
+  value v -> exists v',
+  v = rec l v'.
+Proof.
+  introv Ht. inductions Ht; introv Hv;
+  try solve [inverts* Hv].
+Qed. 
+
+Lemma notin_false: forall E v A,
+  has_type E v A -> forall l v',
+  rlookupv v l v' ->
+  ~ lin l A ->
+  False.
+Proof.
+  introv Ht. inductions Ht; introv Hr Hnl;
+  try solve [inverts* Hr].
+Qed.
+
+Lemma rlookup_pres_aux: forall E l A,
+  rlookup E l A -> forall v v',
+  rlookupv v l v' -> 
+  value v ->
+  has_type top v E ->
+  has_type E v' A.
+Proof.
+  introv Hl. inductions Hl; introv Hlv Hv Ht.
+  - inverts* Ht; try solve [inverts Hv].
+    inverts Hlv. inverts Hv.
+    eapply value_weaken; eauto.
+  - inverts* Hlv; try solve [inverts* Ht]. 
+    + inverts Ht. inverts Hv.
+      forwards~: IHHl H0 H5. 
+      eapply value_weaken; eauto.
+      eapply rlookupv_value; eauto.
+    + inverts Ht. inverts Hv. 
+      exfalso. eapply notin_false; eauto.
+  - inverts* Hlv; try solve [inverts* Ht]. 
+    + inverts Ht. inverts Hv. 
+      exfalso. eapply notin_false; try eapply H; eauto.
+    + inverts Ht. inverts Hv.
+      forwards~: IHHl H0. 
+      eapply value_weaken; eauto.
+      eapply value_weaken; eauto.
+      eapply rlookupv_value; eauto.
+Qed. 
+
+Lemma rlookup_pres: forall E l A,
+  rlookup E l A -> forall v v',
+  rlookupv v l v' -> 
+  value v ->
+  has_type top v E ->
+  has_type top v' A.
+Proof.
+  introv Hl Hlv Hv Ht.
+  forwards~: rlookup_pres_aux Hl Hlv Hv Ht.
+  eapply value_weaken; eauto.
+  eapply rlookupv_value; eauto.
+Qed.
+
+
+Lemma gpreservation : forall e e' v, 
+  step v e e' -> forall E A, 
+  has_type E e A -> 
+  has_type top v E -> 
+  has_type E e' A.
+Proof.
+  introv Hs. inductions Hs; introv Ht Htv; 
+  try solve [eauto];
+  try solve [inverts* Ht].
+  - inverts* Ht.
+    eapply value_weaken; eauto.
+  - inverts* Ht.
+    econstructor; eauto.
+    eapply IHHs; eauto.
+    eapply value_weaken; eauto.
+  - inverts* Ht.
+    econstructor; eauto.
+    eapply IHHs; eauto.
+    econstructor; eauto.
+    eapply value_weaken; eauto.
+  - inverts* Ht. inverts H5.
+    econstructor; eauto.
+    econstructor.
+    eapply value_weaken; eauto.
+    eapply value_weaken; eauto.
+  - inverts* Ht.
+    eapply value_weaken; eauto.
+  - inverts* Ht.
+    forwards~: lookup_pres H7 H1.
+    eapply value_weaken; eauto.
+    eapply value_weaken; eauto.
+    eapply lookupv_value; eauto.
+  - inverts* Ht.
+    forwards~: rlookup_pres H7 H1.
+    eapply value_weaken; eauto.
+    eapply value_weaken; eauto.
+    eapply rlookupv_value; eauto.
+Qed.
+
+    
+Lemma lookup_prog: forall n A B,
+  lookup A n B -> forall v,
+  has_type top v A ->
+  value v ->
+  exists e', lookupv v n e'.
+Proof.
+  introv Hl. inductions Hl; introv Ht Hv.
+  - inverts* Ht; try solve [inverts* Hv].
+  - inverts* Ht; try solve [inverts* Hv].
+    + inverts* Hv. 
+      forwards~ (e'&Hs): IHHl H3.
+      inverts* Hs.
+Qed.
+
+Lemma rlookup_prog: forall n A B,
+  rlookup A n B -> forall v,
+  has_type top v A ->
+  value v ->
+  exists e', rlookupv v n e'.
+Proof.
+  introv Hl. inductions Hl; introv Ht Hv.
+  - inverts* Ht; try solve [inverts* Hv].
+  - inverts* Ht; try solve [inverts* Hv].
+    inverts Hv.
+    forwards~ (?&?): IHHl H4.
+    exists* x.
+  - inverts* Ht; try solve [inverts* Hv].
+    inverts Hv.
+    forwards~ (?&?): IHHl e2.
+    eapply value_weaken; eauto.
+    exists* x.
+Qed.
+
+
+Lemma gprogress : forall E e A, 
+  has_type E e A -> forall v, 
+  value v -> 
+  has_type top v E -> 
+  value e \/ exists e', step v e e'.
+Proof.
+  introv Ht.
+  inductions Ht; introv Hv Htv; eauto.
+  - right. 
+    forwards~: IHHt1 Htv.
+    forwards~: IHHt2 Htv.
+    destruct* H; destruct* H0.
+    + inverts* Ht1; inverts* H.
+  - forwards~: IHHt1 Htv.
+    destruct H.
+    + forwards~: IHHt2 H.
+      eapply value_weaken; eauto.
+      destruct* H0.
+    + inverts* H.
+  - forwards~: IHHt1 Htv.
+    destruct H.
+    + forwards~: IHHt2 (binop mrg v e1).
+      econstructor; eauto.
+      eapply value_weaken; eauto.
+      destruct* H0.
+    + inverts* H.
+  - right.
+    forwards~: IHHt Hv.
+    inverts H0.
+    + forwards~: value_weaken Ht top.
+      forwards~ (?&?): lookup_prog H H0.
+      exists* x.
+    + inverts* H1.
+  - forwards~: IHHt Hv Htv. destruct* H.
+  - right.
+    forwards~: IHHt Hv.
+    inverts H0.
+    + forwards~: value_weaken Ht top.
+      forwards~ (?&?): rlookup_prog H H0.
+      exists* x. 
+    + inverts* H1.
+Qed.
+
+Lemma preservation : forall e e' A, has_type top e A -> step unit e e' -> has_type top e' A.
+  intros.
+  eapply gpreservation; eauto.
+Defined.
+      
+Lemma progress :  forall e A, has_type top e A -> value e \/ exists e', step unit e e'.
+  intros.
+  eapply gprogress; eauto.
+Defined.
+
+
+(* ---------------------------------------------------- *)
+(* Determinism *)
+Lemma step_value : forall e, 
+  value e -> forall v e', 
+  step v e e' -> 
+  False.
+Proof.
+  induction 1; intros v' e' st; dependent destruction st; eauto.
+Qed.
+
+Ltac solve_value_step :=
+  match goal with
+    | [ Hv : value ?v, H : step _ ?v _ |- _ ] => 
+          exfalso; forwards~: step_value Hv H
+    | [ Hv : value ?v, H : step _ (clos ?v _ _) _ |- _ ] => 
+          exfalso; eapply step_value; try eapply H; eauto 
+  end. 
+
+Lemma lookupv_det: forall v n v1,
+  lookupv v n v1 -> forall v2,
+  lookupv v n v2 ->
+  v1 = v2.
+Proof.
+  introv Hl. inductions Hl; introv Hl2; inverts* Hl2.
+Qed.
+
+Inductive mstep : exp -> exp -> exp -> Prop :=
+  | mstep_base : forall v e, value v -> mstep v e e
+  | mstep_step : forall v e e' e'', step v e e' -> mstep v e' e'' -> mstep v e e''.
+
+#[export]
+Hint Constructors mstep: core.
+
+
+Lemma rlookupv_det: forall v E B,
+  has_type E v B ->
+  value v -> forall l A,
+  rlookup B l A -> forall v1,
+  rlookupv v l v1 -> forall v2,
+  rlookupv v l v2 ->
+  v1 = v2.
+Proof.
+  introv Ht. inductions Ht; introv Hv Hr Hl1 Hl2;
+  try solve [inverts Hl1].
+  - inverts Hv. inverts Hr. 
+    + inverts Hl1; inverts Hl2.
+      * eapply IHHt1; eauto.
+      * exfalso. eapply notin_false; eauto.
+      * exfalso. eapply notin_false; eauto.
+      * exfalso. eapply notin_false; eauto.
+    + inverts Hl1; inverts Hl2.
+      * exfalso. eapply notin_false; try eapply H6; eauto.
+      * exfalso. eapply notin_false; try eapply H6; eauto.
+      * exfalso. eapply notin_false; try eapply H6; eauto.
+      * eapply IHHt2; eauto.
+  - inverts Hl1. inverts Hl2. eauto. 
+Qed. 
+
+Lemma sel_det: forall v l E A,
+  has_type E (rproj v l) A ->
+  value v -> forall v1,
+  rlookupv v l v1 -> forall v2,
+  rlookupv v l v2 ->
+  v1 = v2.
+Proof.
+  introv Hs. inverts Hs; intros.
+  eapply rlookupv_det; eauto.
+Qed.
+
+
+Lemma gen_step_unique: forall e A G, 
+  has_type G e A -> forall v e1 e2, 
+  has_type top v G -> 
+  step v e e1 ->
+  step v e e2 -> 
+  e1 = e2.
+Proof.
+  intros e A G H.
+  inductions H; introv Typv Red1 Red2;
+  try solve [inverts Red1].
+  - inverts* Red1. inverts* Red2.
+  - inverts Red1; inverts Red2; 
+    try solve_value_step.
+    + forwards~: IHhas_type1 H7 H9. subst. eauto.
+    + forwards~: IHhas_type2 H7 H10. subst. eauto.
+    + eauto.
+  - inverts Red1; inverts Red2; 
+    try solve_value_step.
+    + forwards~: IHhas_type1 H7 H9. subst. eauto.
+    + forwards~: IHhas_type2 H7 H10. 
+      eapply value_weaken; eauto.
+      subst. eauto.
+    + eauto.
+  - inverts Red1; inverts Red2; 
+    try solve_value_step.
+    + forwards~: IHhas_type1 H7 H9. subst. eauto.
+    + forwards~: IHhas_type2 H7 H10.
+      econstructor; eauto. 
+      eapply value_weaken; eauto.
+      subst. eauto.
+  - inverts Red1; inverts Red2. eauto.
+  - inverts Red1; inverts Red2; 
+    try solve_value_step.
+    + forwards~: IHhas_type H6 H8. subst. eauto.
+    + eapply lookupv_det; eauto.
+  - inverts Red1; inverts Red2; 
+    try solve_value_step.
+    + forwards~: IHhas_type H5 H7. subst. eauto.
+  - inverts Red1; inverts Red2; 
+    try solve_value_step.
+    + forwards~: IHhas_type H6 H8. subst. eauto.
+    + eapply rlookupv_det; try eapply H7; eauto.
+Qed.
+
+
+Corollary step_unique: forall e A, 
+  has_type top e A -> forall e1 e2, 
+  step unit e e1 ->
+  step unit e e2 -> 
+  e1 = e2.
+Proof.
+  introv Ht Hs1 Hs2.
+  forwards~: gen_step_unique Ht Hs1 Hs2.
+Qed.
+
+
+
+Lemma mstep_trans : forall v e1 e2, 
+  mstep v e1 e2 -> forall e3, 
+  mstep v e2 e3 -> 
+  mstep v e1 e3.
+  intros v e1 e2 ms.
+  induction ms; intros e3 ms2; eauto.
+Defined.
+
+
+Lemma mstep_det: forall v e v1,
+  mstep v e v1 -> forall v2,
+  mstep v e v2 -> forall A G, 
+  has_type G e A ->  
+  has_type top v G -> 
+  value v1 ->
+  value v2 ->
+  v1 = v2.
+Proof.
+  introv Hm. inductions Hm; introv Hm2 Ht Hs Hv1 Hv2.
+  - inductions Hm2; eauto.
+    exfalso. forwards~: step_value H0.
+  - inverts Hm2; eauto.
+    + exfalso. forwards~: step_value H.
+    + forwards~: gen_step_unique Ht Hs H H0. subst.
+      eapply IHHm; eauto.
+      eapply gpreservation; eauto.
+Qed.
+
+
+(* ---------------------------------------------------- *)
+(* Termination *)
+
+
+Fixpoint sem_typ_val (e: exp) (A : typ) : Prop :=
+  match A with
+  | top => e = unit 
+  | int => exists i, e = lit i 
+  | and B1 B2 => exists v1 v2, e = binop mrg v1 v2 /\ sem_typ_val v1 B1 /\ sem_typ_val v2 B2
+  | arr B1 B2 => exists v e', 
+      value v /\ e = clos v B1 e' /\
+        (forall v1, value v1 -> sem_typ_val v1 B1 -> exists v2,
+                    (mstep unit (binop box (binop mrg v v1) e') v2) /\ sem_typ_val v2 B2) 
+  | rcd l A => exists v, e = rec l v /\ sem_typ_val v A
+  end.
+
+
+Lemma stv_value : forall A e, sem_typ_val e A -> value e.
+  induction A; simpl in *; intros; eauto.
+  - destruct H; subst; eauto.
+  - subst; eauto.
+  - destruct H as (? & ? & ? & ? & ?); subst; eauto.
+  - destruct H as (? & ? & ? & ? & ?); subst; eauto.
+  - destruct H as (? & ? & ?); subst; eauto.
+Defined.
+
+Lemma sem_lookup_preservation : forall A n B, 
+  lookup A n B -> forall v v',
+  lookupv v n v' -> 
+  value v -> 
+  sem_typ_val v A -> 
+  sem_typ_val v' B.
+  intros A n B l.
+  induction l; intros; eauto; dependent destruction H; dependent destruction H0; simpl in *; eauto.
+  - destruct H1. destruct H. destruct H. destruct H0.
+    injection H; intros; subst; eauto.
+  - destruct H1. destruct H0. destruct H0. destruct H1.
+    injection H0; intros; subst; eauto.    
+Defined.
+
+
+Lemma notin_false_sem: forall A v,
+  sem_typ_val v A -> 
+  value v -> forall l v',
+  rlookupv v l v' ->
+  ~ lin l A ->
+  False.
+Proof.
+  intros A. inductions A; introv Hs Hv;
+  try solve [inverts* Hv]; intros.
+  - simpl in Hs. destruct* Hs. subst*. inverts* H. 
+  - simpl in Hs. subst*. inverts* H.
+  - simpl in Hs.
+    destruct Hs. destruct H1.
+    destruct H1. destruct H2. subst. inverts H.
+  - simpl in Hs.
+    destruct Hs. destruct H1.
+    destruct H1. destruct H2. subst. inverts Hv. inverts* H.
+  - simpl in Hs.
+    destruct Hs. destruct H1. subst. inverts H. 
+    eapply H0. eauto.
+Qed.
+
+Lemma sem_rlookup_preservation : forall A n B, 
+  rlookup A n B -> forall v v',
+  rlookupv v n v' -> 
+  value v -> 
+  sem_typ_val v A -> 
+  sem_typ_val v' B.
+Proof.
+  introv Hl. inductions Hl; introv Hlv Hv Ht.
+  - simpl in Ht. forwards~ (?&?&?): Ht.
+    subst*. inverts* Hlv.
+  - simpl in Ht. forwards~ (?&?&?&?&?): Ht.
+    subst*. inverts* Hlv.
+    + eapply IHHl; eauto.
+      eapply stv_value; eauto.
+    + exfalso. eapply notin_false_sem; eauto.
+      eapply stv_value; eauto.
+  - simpl in Ht. forwards~ (?&?&?&?&?): Ht.
+  subst*. inverts* Hlv.
+    + exfalso. eapply notin_false_sem; try eapply H; eauto.
+    eapply stv_value; eauto.
+    + eapply IHHl; eauto.
+      eapply stv_value; eauto.
+Defined.
+
+Definition comp_env (o : op) (v v1 : exp) : exp :=
+  match o with
+  | mrg => binop mrg v v1
+  | box => v1
+  | _ => v 
+  end.
+
+Lemma mstep_value: forall v venv v',
+  mstep venv v v' ->
+  value v ->
+  v = v'.
+Proof.
+  introv Hm. inductions Hm; introv Hv; eauto.
+  exfalso. eapply step_value; eauto.
+Qed.
+
+Lemma weaken_box : forall v e1 e2 e, 
+  value e1 -> 
+  mstep v (binop box e1 e2) e -> forall v', 
+  value v' -> 
+  mstep v' (binop box e1 e2) e.
+  intros.
+  dependent induction H0; eauto.
+  dependent destruction H1; eauto.
+  apply step_value in H1; eauto. inversion H1.
+  rewrite (mstep_value _ _ _ H2) in *; eauto.
+Defined.
+
+Lemma sound_lookup : forall A n B, 
+  lookup A n B -> forall v, 
+  sem_typ_val v A -> exists v', 
+  lookupv v n v'.
+  induction 1; simpl; intros v sv; eauto.
+  - destruct sv as (? & ? & ? & ? & ?). subst; eauto.
+  - destruct sv as (? & ? & ? & ? & ?). subst; eauto.
+    apply IHlookup in H1. destruct H1. exists x1. eauto.
+Defined.
+
+Lemma mstep_split : forall v e1 v1, mstep v e1 v1 -> value v -> value v1 ->
+                                     forall e2 e2' o, mstep (comp_env o v v1) e2 e2' -> mstep v (binop o e1 e2) (binop o v1 e2').
+  intros v e1 v1 ms. induction ms; intros valv valv1 e2 e2' o ms2; eauto.
+  dependent induction ms2; eauto.
+  destruct o; simpl; eauto.
+Defined.
+
+Lemma step_env_value: forall v e1 e2,
+  step v e1 e2 ->
+  value v.
+Proof.
+  introv Hs. inductions Hs; eauto.
+Qed.
+
+Lemma mstep_env_value: forall v e1 e2,
+  mstep v e1 e2 ->
+  value v.
+Proof.
+  introv Hs. inductions Hs; eauto.
+Qed.
+
+Lemma step_is_mstep: forall v e1 e2,
+  step v e1 e2 ->
+  mstep v e1 e2.
+Proof.
+  introv Hs. econstructor; eauto.
+  eapply mstep_base; eauto.
+  eapply step_env_value; eauto.
+Qed.
+
+Lemma mstep_rec: forall v e1 e2 l,
+  mstep v e1 e2 -> 
+  mstep v (rec l e1) (rec l e2).
+Proof.
+  introv Hm.
+  inductions Hm; eauto.
+  eapply mstep_trans; eauto.
+  eapply step_is_mstep; eauto.
+  econstructor; eauto.
+  eapply step_env_value; eauto.
+Qed.
+
+Lemma sound_rlookup : forall A n B, 
+  rlookup A n B -> forall v, 
+  sem_typ_val v A -> exists v', 
+  rlookupv v n v'.
+  induction 1; simpl; intros v sv; eauto.
+  - destruct sv as (? & ? & ?). subst; eauto.
+  - destruct sv as (? & ? & ? & ? & ?). subst; eauto.
+    forwards~ (?&?): IHrlookup H2. exists*.
+  - destruct sv as (? & ? & ? & ? & ?). subst; eauto.
+    forwards~ (?&?): IHrlookup H3. exists*.
+Defined.
+
+Lemma mstep_rproj: forall v e1 e2 l,
+  mstep v e1 e2 -> 
+  mstep v (rproj e1 l) (rproj e2 l).
+Proof.
+  introv Hm.
+  inductions Hm; eauto.
+  eapply mstep_trans; eauto.
+  eapply step_is_mstep; eauto.
+  econstructor; eauto.
+  eapply step_env_value; eauto.
+Qed.
+
+Lemma mstep_proj: forall v e1 e2 n,
+  mstep v e1 e2 -> 
+  mstep v (proj e1 n) (proj e2 n).
+Proof.
+  introv Hm.
+  inductions Hm; eauto.
+  eapply mstep_trans; eauto.
+  eapply step_is_mstep; eauto.
+  econstructor; eauto.
+  eapply step_env_value; eauto.
+Qed.
+
+Definition sem_typ (E : typ) (e : exp) (A : typ) : Prop := forall venv,
+  sem_typ_val venv E ->
+  exists v, mstep venv e v /\ sem_typ_val v A.
+
+
+Ltac pre_unfold :=
+  unfold sem_typ; 
+  introv msv; 
+  match goal with
+    | [ msv : _ |- _ ] => 
+      try forwards~ Hv: stv_value msv
+  end. 
+
+Lemma sound_ctx: forall E,
+  sem_typ E ctx E.
+Proof.
+  pre_unfold. exists* venv.
+Qed.
+
+Lemma sound_box: forall E e1 E1 e2 A,
+  sem_typ E e1 E1 ->
+  sem_typ E1 e2 A ->
+  sem_typ E (binop box e1 e2) A.
+Proof.
+  introv IHht1 IHht2. pre_unfold.
+  destruct (IHht1 _ msv) as (? & ? & ?).
+  assert (value venv). eapply stv_value; eauto.
+  assert (value x). eapply stv_value; eauto.
+  unfold sem_typ in *.
+  destruct (IHht2 _ H0) as (? & ? & ?); simpl.
+  exists x0. split; eauto.
+  assert (value x0). eapply stv_value; eauto.
+  apply mstep_trans with (e2 := binop box x x0); eauto.
+  apply mstep_split; eauto.
+Qed.
+
+
+Lemma sound_lam: forall E A e B,
+  sem_typ (and E A) e B ->
+  sem_typ E (lam A e) (arr A B).
+Proof.
+  introv IHht. pre_unfold.
+  exists (clos venv A e). split; eauto.
+  simpl. exists venv. exists e. split; eauto. split; eauto.
+  intros.
+  destruct (IHht (binop mrg venv v1)).
+  simpl. exists venv. exists v1. repeat (split; eauto).
+  destruct H1. exists x. split; eauto.
+  assert (value x). eapply stv_value; eauto.
+  apply mstep_trans with (e2 := binop box (binop mrg venv v1) x); eauto.
+  apply mstep_split; eauto.
+Qed.
+
+
+Lemma soundness : forall e A E, 
+  has_type E e A -> 
+  sem_typ E e A.
+Proof.
+  introv ht. inductions ht.
+  - eapply sound_ctx.
+  - pre_unfold. 
+    exists (lit i); split; unfold sem_typ_val; eauto.
+  - pre_unfold.
+    exists unit; split; unfold sem_typ_val; eauto.
+  - pre_unfold. 
+    destruct (IHht1 _ msv). destruct (IHht2 _ msv).
+    destruct H0. destruct H.
+    simpl in H2.
+    destruct H2 as (? & ? & ? & ? & ?). subst.
+    assert (value x0). eapply stv_value; eauto.
+    edestruct H4 as (? & ? & ?); eauto.
+    apply weaken_box with (v' := venv) in H5; eauto.    
+    exists x. split; eauto.
+    eapply mstep_trans; try (exact H5).
+    eapply mstep_trans with (e2 := binop app (clos x1 A x2) x0); eauto.
+    apply mstep_split; eauto.
+  - eapply sound_box; eauto.
+  - pre_unfold.
+    destruct (IHht1 _ msv) as (? & ? & ?).
+    unfold sem_typ in *.
+    assert (value venv). eapply stv_value; eauto.
+    assert (value x). eapply stv_value; eauto.
+    destruct (IHht2 (binop mrg venv x)) as (? & ? & ?); simpl.
+    exists venv. exists x. split; eauto.
+    exists (binop mrg x x0). split; eauto.    
+    apply mstep_split; eauto.
+  - eapply sound_lam; eauto. 
+  - pre_unfold.
+    forwards~ (?&?&?): IHht msv.
+    forwards~ (?&?): sound_lookup H H1.    
+    forwards~: sem_lookup_preservation H H2 H1.
+    eapply stv_value; eauto.
+    exists* x0. split*.
+
+    eapply mstep_trans.
+    + eapply mstep_proj; eauto.
+    + eapply step_is_mstep. econstructor; eauto.
+      eapply stv_value; eauto.
+  - pre_unfold.
+    exists (clos ev A e). split; simpl; eauto.
+    exists ev. exists e. split; eauto. split; eauto.
+    intros.
+
+    destruct (IHht1 unit); simpl; eauto. destruct H2.
+    destruct (IHht2 (binop mrg ev v1)).
+    forwards~: mstep_value H2. subst.
+    simpl. exists x. exists v1. repeat (split; eauto).
+    destruct H4. exists x0; split; eauto.
+    assert (value x0). eapply stv_value; eauto.
+    apply mstep_trans with (e2 := binop box (binop mrg ev v1) x0); eauto.
+    apply mstep_split; eauto. 
+  - pre_unfold.
+    forwards~ (?&?&?): IHht msv. exists* (rec l x). split*.
+    + eapply mstep_rec; eauto.
+    + simpl. exists*.
+  - pre_unfold.
+    forwards~ (?&?&?): IHht msv.
+    forwards~ (?&?): sound_rlookup H H1.    
+    forwards~: sem_rlookup_preservation H H2 H1.
+    eapply stv_value; eauto.
+    exists* x0. split*.
+
+    eapply mstep_trans.
+    + eapply mstep_rproj; eauto.
+    + eapply step_is_mstep. econstructor; eauto.
+      eapply stv_value; eauto.
+Qed.
+
+
+Lemma termination : forall e A, has_type top e A -> exists v, value v /\ mstep unit e v.
+Proof.
+  intros.
+  apply soundness with (E := top) in H; simpl; eauto.
+  unfold sem_typ in H.
+  forwards~ (?&?&?): H unit. exists x. split*.
+  eapply stv_value; eauto.
+Qed.
